schema/Pages.v
@@ -1,6 +1,9 @@
 From Stdlib Require Import String.
 From Stdlib Require Import Ascii.
-Require Import Proj.Cabs.
+From Stdlib Require Import List.
+
+Definition id_size := 1.
+Definition name_size := 32. (*Cans be 32 ascii*)
 
 Parameter pages_type : Type.
 
@@ -17,5 +20,23 @@ Record row := {
   name : string
 }.
 
-Extract Constant Pages.pages_type => "Bytes.t option array".
+Definition deserialize_row (b : list ascii) : row :=
+  match b with
+  | id :: name => {| id := id; name := string_of_list_ascii name |}
+  | nil => {| id := "0"%char; name := "" |}  (* or handle differently if needed *)
+  end.
 
+Definition serialize_row (r : row) : list ascii :=
+  r.(id) :: list_ascii_of_string r.(name).
+
+Theorem serializing_inv : forall (r : row) (s : list ascii), s <> nil -> deserialize_row (serialize_row r) = r 
+  /\ serialize_row(deserialize_row s) = s.
+Proof.
+split. simpl. rewrite string_of_list_ascii_of_string. destruct r. simpl. reflexivity.
+induction s. exfalso. apply H. reflexivity. unfold serialize_row. simpl. rewrite list_ascii_of_string_of_list_ascii.
+reflexivity.
+Qed.
+
+Require Import ExtrOcamlBasic.
+Require Import ExtrOcamlString.
+Extract Constant pages_type => "Bytes.t option array".
